Adding a potential course file

fstar/Logos/Logos.fst
@@ -3,23 +3,40 @@ module Logos
 
 open FStar.List
 open FStar.Nat
-open FStar.String 
-open FStar.Maybe
- 
-type ty = | Int : ty
+open FStar.String
+open FStar.All
+(* open FStar.Maybe *)
+
+type atom = string
+
+val === : atom -> atom -> bool
+
+type ty = 
+  | Int : ty
   | Str : ty 
-  | Sort : string -> nat : ty 
+  | Sort : atom -> ty 
   | Rel : ty -> ty -> ty 
   | Pi : ty -> ty 
-  | TyVar : string -> nat -> ty
+  | TyVar : atom -> nat -> ty
 
-type term = | Var : string -> nat -> term 
-  | Funsym : string -> (list term) -> term
+type term = 
+  | Var : atom -> term 
+  | Funsym : atom -> (list term) -> term
   
-type log = | And : log -> log -> log
+type log = 
+  | And : log -> log -> log
   | Or : log -> log -> log
   | Lam : log -> log -> log
   | Term : term -> log
 
-unify : term -> term -> maybe term
+type subst = list (term * term)
 
+val fv : s:term -> nat 
+let rec fv s ex = match s with
+ | Var a -> 
+
+val unify: theta:subst -> s:term -> t:term -> Tot (option term)
+unify (
+
+
+(* let rec unify t s = *)
