agda/Course/OperationalSemantics.agda
@@ -1,0 +1,186 @@
+
+module OperationalSemantics where
+
+open import Data.Nat
+
+data E : Set where
+  num : ℕ → E
+  _⊕_ : E → E → E
+  _⊗_ : E → E → E
+
+-- Big step operational semantics
+
+infix 10 _⇓_ 
+data _⇓_ : E → E → Set where
+  n⇓n : ∀ n →
+
+      -------------
+      num n ⇓ num n
+      
+  E⊕E : ∀ E₁ E₂ n₁ n₂ →
+  
+      E₁ ⇓ num n₁ → E₂ ⇓ num n₂ →
+      ---------------------------------
+         E₁ ⊕ E₂ ⇓ num (n₁ + n₂)
+  
+  E⊗E : ∀ E₁ E₂ n₁ n₂ →
+  
+      E₁ ⇓ num n₁ → E₂ ⇓ num n₂ →
+      ---------------------------------
+         E₁ ⊗ E₂ ⇓ num (n₁ * n₂)
+
+-- Need for Σ which gives us specifications / existentials.
+open import Data.Product
+
+-- Σ[ n ∈ ℕ ] P
+-- We can read this as: There exists an n in ℕ such that P
+---
+-- It is a type of pairs, which has a witness (of type ℕ in this case) and a proof
+-- that P holds of that witness.
+--
+evalBig : ∀ E → Σ[ n ∈ ℕ ] E ⇓ num n
+evalBig (num x) = x , n⇓n x
+evalBig (e ⊕ e₁) with evalBig e | evalBig e₁
+evalBig (e ⊕ e₁) | n , proof_n | m , proof_m = n + m , E⊕E e e₁ n m proof_n proof_m
+evalBig (e ⊗ e₁) with evalBig e | evalBig e₁
+evalBig (e ⊗ e₁) | n , proof_n | m , proof_m = n * m , E⊗E e e₁ n m proof_n proof_m
+
+example⇓ : num 3 ⊕ (num 2 ⊕ num 1) ⇓ num 6
+example⇓ = proj₂ (evalBig (num 3 ⊕ (num 2 ⊕ num 1)))
+
+-- Small step operational semantics
+infix 8 _⟶_
+data _⟶_ : E → E → Set where
+  +⟶ : ∀ n m →
+  
+          -----------------------------
+          num n ⊕ num m ⟶ num (n + m)
+
+  *⟶ : ∀ n m →
+  
+          -----------------------------
+          num n ⊗ num m ⟶ num (n * m)
+
+  ⊕₁⟶ : ∀ E₁ E₁' E₂ →
+
+          E₁ ⟶ E₁' → 
+          ---------------------
+          E₁ ⊕ E₂ ⟶ E₁' ⊕ E₂
+
+  ⊕₂⟶ : ∀ n E₂ E₂' →
+
+          E₂ ⟶ E₂' →  
+          --------------------
+          num n ⊕ E₂ ⟶ num n ⊕ E₂'
+
+  ⊗₁⟶ : ∀ E₁ E₁' E₂ →
+
+          E₁ ⟶ E₁' → 
+          ---------------------
+          E₁ ⊗ E₂ ⟶ E₁' ⊗ E₂
+
+  ⊗₂⟶ : ∀ n E₂ E₂' →
+
+          E₂ ⟶ E₂' → 
+          ---------------------
+          num n ⊗ E₂ ⟶ num n ⊗ E₂'
+
+example⟶₁ : (num 3 ⊕ num 7) ⊕ (num 8 ⊕ num 1) ⟶ num 10 ⊕ (num 8 ⊕ num 1)
+example⟶₁ = ⊕₁⟶ _ _ _ (+⟶ 3 7)
+example⟶₂ : (num 10) ⊕ (num 8 ⊕ num 1) ⟶ num 10 ⊕ num 9
+example⟶₂ = ⊕₂⟶ _ _ _ (+⟶ 8 1)
+
+infix 8 _⟶ch_
+data _⟶ch_ : E → E → Set where
+  +⟶ch : ∀ n m →
+  
+          -----------------------------
+          num n ⊕ num m ⟶ch num (n + m)
+
+  *⟶ch : ∀ n m →
+  
+          -----------------------------
+          num n ⊗ num m ⟶ch num (n * m)
+
+  ⊕₁⟶ch : ∀ E₁ E₁' E₂ →
+
+          E₁ ⟶ch E₁' → 
+          ---------------------
+          E₁ ⊕ E₂ ⟶ch E₁' ⊕ E₂
+
+  ⊕₂⟶ch : ∀ E₁ E₂ E₂' →
+
+          E₂ ⟶ch E₂' →  
+          --------------------
+          E₁ ⊕ E₂ ⟶ch E₁ ⊕ E₂'
+
+  ⊗₁⟶ch : ∀ E₁ E₁' E₂ →
+
+          E₁ ⟶ch E₁' → 
+          ---------------------
+          E₁ ⊗ E₂ ⟶ch E₁' ⊗ E₂
+
+  ⊗₂⟶ch : ∀ E₁ E₂ E₂' →
+
+          E₂ ⟶ch E₂' → 
+          ---------------------
+          E₁ ⊗ E₂ ⟶ch E₁ ⊗ E₂'
+
+example⟶ch₁ : (num 3 ⊕ num 7) ⊕ (num 8 ⊕ num 1) ⟶ch num 10 ⊕ (num 8 ⊕ num 1)
+example⟶ch₁ = ⊕₁⟶ch _ _ _ (+⟶ch 3 7)
+example⟶ch₂ : (num 10) ⊕ (num 8 ⊕ num 1) ⟶ch num 10 ⊕ num 9
+example⟶ch₂ = ⊕₂⟶ch _ _ _ (+⟶ch 8 1)
+
+⟶⇒⟶ch : ∀ {E₁ E₂} → (E₁ ⟶ E₂) → (E₁ ⟶ch E₂)
+⟶⇒⟶ch (+⟶ n m) = +⟶ch n m
+⟶⇒⟶ch (*⟶ n m) = *⟶ch n m
+⟶⇒⟶ch (⊕₁⟶ E₁ E₁' E₂ d) = ⊕₁⟶ch E₁ E₁' E₂ (⟶⇒⟶ch d)
+⟶⇒⟶ch (⊕₂⟶ n E₂ E₂' d) = ⊕₂⟶ch (num n) E₂ E₂' (⟶⇒⟶ch d)
+⟶⇒⟶ch (⊗₁⟶ E₁ E₁' E₂ d) = ⊗₁⟶ch E₁ E₁' E₂ (⟶⇒⟶ch d)
+⟶⇒⟶ch (⊗₂⟶ n E₂ E₂' d) = ⊗₂⟶ch (num n) E₂ E₂' (⟶⇒⟶ch d)
+
+{- Not a theorem! -}
+⟶ch⇒⟶ : ∀ {E₁ E₂} → (E₁ ⟶ch E₂) → (E₁ ⟶ E₂)
+⟶ch⇒⟶ (+⟶ch n m) = +⟶ n m
+⟶ch⇒⟶ (*⟶ch n m) = *⟶ n m
+⟶ch⇒⟶ (⊕₁⟶ch E₁ E₁' E₂ d) = ⊕₁⟶ E₁ E₁' E₂ (⟶ch⇒⟶ d)
+⟶ch⇒⟶ (⊕₂⟶ch E₁ E₂ E₂' d) = {!!} {-  E₂ ⟶ E₂'                  No applicable rule
+                                           ———————————————————             
+                                           (E₁ ⊕ E₂) ⟶ (E₁ ⊕ E₂')  -}
+⟶ch⇒⟶ (⊗₁⟶ch E₁ E₁' E₂ d) = ⊗₁⟶ E₁ E₁' E₂ (⟶ch⇒⟶ d)
+⟶ch⇒⟶ (⊗₂⟶ch E₁ E₂ E₂' d) = {!!} {-  E₂ ⟶ E₂'                  No applicable rule
+                                           ———————————————————             
+                                           (E₁ ⊗ E₂) ⟶ (E₁ ⊗ E₂')  -}
+
+data _⟶_⟨_⟩ : E → E → ℕ → Set where
+  z⟶ : ∀ E₁ →
+  
+                 --------------
+                 E₁ ⟶ E₁ ⟨ 0 ⟩
+                 
+  sn⟶ : ∀ E₁ E₂ E₃ n →
+
+                 E₁ ⟶ E₂ ⟨ n ⟩  →  E₂ ⟶ E₃ →
+                 -----------------------------
+                 E₁ ⟶ E₃ ⟨ 1 + n ⟩ 
+
+
+data _⟶⋆_ : E → E → Set where
+  k⟶⋆ : ∀ E₁ E₂ →
+
+                 Σ[ k ∈ ℕ ] E₁ ⟶ E₂ ⟨ k ⟩ →
+                 --------------------------
+                 E₁ ⟶⋆ E₂ 
+
+_FinalAnswerOf_ : ℕ → E → Set
+_FinalAnswerOf_ n E = E ⟶⋆ num n
+
+-- We need a notion of equality - we'll use Agda's 
+open import Relation.Binary.PropositionalEquality
+
+⇓Consistency : ∀ {E n m} → (E ⇓ n) × (E ⇓ m) → n ≡ m
+⇓Consistency (n⇓n n , n⇓n .n) = refl
+⇓Consistency (E⊕E E₁ E₂ n₃ n₄ d₁ d₂ , E⊕E .E₁ .E₂ n₁ n₂ d₃ d₄) with ⇓Consistency (d₁ , d₃) | ⇓Consistency (d₂ , d₄)
+⇓Consistency (E⊕E E₁ E₂ n₁ n₂ d₁ d₂ , E⊕E .E₁ .E₂ .n₁ .n₂ d₃ d₄) | refl | refl = refl 
+⇓Consistency (E⊗E E₁ E₂ n₃ n₄ d₁ d₂ , E⊗E .E₁ .E₂ n₁ n₂ d₃ d₄) with ⇓Consistency (d₁ , d₃) | ⇓Consistency (d₂ , d₄)
+⇓Consistency (E⊗E E₁ E₂ n₁ n₂ d₁ d₂ , E⊗E .E₁ .E₂ .n₁ .n₂ d₃ d₄) | refl | refl = refl 
